cont.

Experiments/State_Preamble.thy
@@ -262,6 +262,98 @@ value "d_states m_ex_H 5 2"
 value "d_states m_ex_H 5 3"
 value "d_states m_ex_H 5 4"
 
+(* Version of d_states' without early cutoff for q0 *)
+fun d_states'' :: "(('a \<times> 'b) \<Rightarrow> ('c \<times> 'a) set) \<Rightarrow> 'a \<Rightarrow> 'a \<Rightarrow> 'b list \<Rightarrow> 'a list \<Rightarrow> 'a set \<Rightarrow> nat \<Rightarrow> ('a \<times> 'b) list \<Rightarrow> ('a \<times> 'b) list" where
+  "d_states'' f q q0 inputList nodeList nodeSet 0 m = (case find (\<lambda> x . f (q0,x) \<noteq> {} \<and> (\<forall> (y,q'') \<in> f (q0,x) . (q'' \<in> nodeSet))) inputList of 
+      Some x \<Rightarrow> m@[(q0,x)] |
+      None   \<Rightarrow> m)" |
+  "d_states'' f q q0 inputList nodeList nodeSet (Suc k) m = 
+    (case find_remove_2 (\<lambda> q' x . f (q',x) \<noteq> {} \<and> (\<forall> (y,q'') \<in> f (q',x) . (q'' \<in> nodeSet))) nodeList inputList
+      of None            \<Rightarrow> m |
+         Some (q',x,nodeList') \<Rightarrow> d_states'' f q q0 inputList nodeList' (insert q' nodeSet) k (m@[(q',x)]))"
+
+lemma d_states''_d_states' :
+  assumes "q0 \<notin> set nodeList"
+  shows "(\<exists> qx \<in> set (d_states' f q q0 inputList nodeList nodeSet k m) . fst qx = q0)
+   \<or> (d_states' f q q0 inputList nodeList nodeSet k m = d_states'' f q q0 inputList (q0#nodeList) nodeSet k m)" 
+using assms proof (induction k arbitrary: nodeList nodeSet m)
+  case 0
+  then show ?case by auto
+next
+  case (Suc k)
+  show ?case proof (cases "find (\<lambda> x . f (q0,x) \<noteq> {} \<and> (\<forall> (y,q'') \<in> f (q0,x) . (q'' \<in> nodeSet))) inputList")
+    case None
+    then have *: "find_remove_2 (\<lambda> q' x . f (q',x) \<noteq> {} \<and> (\<forall> (y,q'') \<in> f (q',x) . (q'' \<in> nodeSet))) (q0#nodeList) inputList
+                  = find_remove_2' (\<lambda>q' x. f (q', x) \<noteq> {} \<and> (\<forall>(y, q'')\<in>f (q', x). q'' \<in> nodeSet)) nodeList inputList [q0]"
+      by auto
+    have **: "find_remove_2 (\<lambda> q' x . f (q',x) \<noteq> {} \<and> (\<forall> (y,q'') \<in> f (q',x) . (q'' \<in> nodeSet))) nodeList inputList
+                  = find_remove_2' (\<lambda>q' x. f (q', x) \<noteq> {} \<and> (\<forall>(y, q'')\<in>f (q', x). q'' \<in> nodeSet)) nodeList inputList []"
+      by auto
+
+    show ?thesis proof (cases "find_remove_2 (\<lambda> q' x . f (q',x) \<noteq> {} \<and> (\<forall> (y,q'') \<in> f (q',x) . (q'' \<in> nodeSet))) nodeList inputList")
+      case None
+      then have "find_remove_2 (\<lambda> q' x . f (q',x) \<noteq> {} \<and> (\<forall> (y,q'') \<in> f (q',x) . (q'' \<in> nodeSet))) (q0#nodeList) inputList = None"
+        unfolding * ** using find_remove_2'_diff_prev_None by force
+      then show ?thesis using None \<open>find (\<lambda>x. f (q0, x) \<noteq> {} \<and> (\<forall>(y, q'')\<in>f (q0, x). q'' \<in> nodeSet)) inputList = None\<close> by auto
+    next
+      case (Some a)
+      then obtain q' x nodeList' where a1: "find_remove_2 (\<lambda> q' x . f (q',x) \<noteq> {} \<and> (\<forall> (y,q'') \<in> f (q',x) . (q'' \<in> nodeSet))) nodeList inputList = Some (q',x,nodeList')"
+        by (metis prod_cases3)
+      then obtain nodeList'' where a2: "find_remove_2 (\<lambda> q' x . f (q',x) \<noteq> {} \<and> (\<forall> (y,q'') \<in> f (q',x) . (q'' \<in> nodeSet))) (q0#nodeList) inputList = Some (q',x,nodeList'')"
+        unfolding * ** using find_remove_2'_diff_prev_Some
+      proof -
+        assume a1: "\<And>nodeList''. find_remove_2' (\<lambda>q' x. f (q', x) \<noteq> {} \<and> (\<forall>(y, q'')\<in>f (q', x). q'' \<in> nodeSet)) nodeList inputList [q0] = Some (q', x, nodeList'') \<Longrightarrow> thesis"
+        assume "find_remove_2' (\<lambda>q' x. f (q', x) \<noteq> {} \<and> (\<forall>(y, q'')\<in>f (q', x). q'' \<in> nodeSet)) nodeList inputList [] = Some (q', x, nodeList')"
+        then show ?thesis
+          using a1 by (meson find_remove_2'_diff_prev_Some)
+      qed
+
+      have "d_states' f q q0 inputList nodeList nodeSet (Suc k) m = d_states' f q q0 inputList nodeList' (insert q' nodeSet) k (m@[(q',x)])"
+        using None a1 by auto
+
+      have "d_states'' f q q0 inputList (q0#nodeList) nodeSet (Suc k) m = d_states'' f q q0 inputList nodeList'' (insert q' nodeSet) k (m@[(q',x)])"
+        using None a2 by auto
+
+      have "nodeList'' = (q0 # nodeList')" and "q0 \<notin> set nodeList'"
+        using find_remove_2_set(2,6)[OF a1] find_remove_2_set(6)[OF a2] Suc.prems
+        by auto 
+
+      show ?thesis proof (cases "(\<exists>qx\<in>set (d_states' f q q0 inputList nodeList' (insert q' nodeSet) k (m @ [(q', x)])). fst qx = q0)")
+        case True
+        then show ?thesis using \<open>d_states' f q q0 inputList nodeList nodeSet (Suc k) m = d_states' f q q0 inputList nodeList' (insert q' nodeSet) k (m@[(q',x)])\<close> by auto
+      next
+        case False
+        then have "d_states' f q q0 inputList nodeList' (insert q' nodeSet) k (m @ [(q', x)]) = d_states'' f q q0 inputList (q0 # nodeList') (insert q' nodeSet) k (m @ [(q', x)])"
+          using Suc.IH[of nodeList' "insert q' nodeSet" "m@[(q',x)]", OF \<open>q0 \<notin> set nodeList'\<close>] by blast
+        then show ?thesis 
+          unfolding \<open>d_states' f q q0 inputList nodeList nodeSet (Suc k) m = d_states' f q q0 inputList nodeList' (insert q' nodeSet) k (m@[(q',x)])\<close>
+                    \<open>d_states'' f q q0 inputList (q0#nodeList) nodeSet (Suc k) m = d_states'' f q q0 inputList nodeList'' (insert q' nodeSet) k (m@[(q',x)])\<close> 
+                    \<open>nodeList'' = (q0 # nodeList')\<close>
+          by blast
+      qed
+        
+    qed
+  next
+    case (Some x)
+
+    moreover have "find_remove_2 (\<lambda> q' x . f (q',x) \<noteq> {} \<and> (\<forall> (y,q'') \<in> f (q',x) . (q'' \<in> nodeSet))) (q0#nodeList) inputList = Some (q0,x,nodeList)"
+      unfolding find_remove_2.simps find_remove_2'.simps Some
+      by simp
+
+    ultimately show ?thesis by auto
+  qed
+qed
+
+
+
+
+
+(* TODO: use d_states'' for proofs ? *)
+
+end (*
+
+
+
 (*
 fun d_states_old :: "('a::linorder,'b::linorder,'c) fsm \<Rightarrow> nat \<Rightarrow> 'a \<Rightarrow> ('a \<times> 'b) list" where
   "d_states_old M 0 q = []" |
@@ -1651,6 +1743,11 @@ qed
 
 
 
+
+
+
+
+end (*
 
 
 
